Code/Examples/Map.v
@@ -38,45 +38,37 @@ Definition Cons {C} : tm map_ar C _ := BaseTm TCons.
 Definition Map {C} : tm map_ar C _ := BaseTm TMap.
 
 (** The rewrite rules *)
-Definition map_nil
-  : rewriteRule map_ar
-  := make_rewrite
-       (_ ,, ∙) _
-       (let f := TmVar Vz in
-        Map · f · Nil)
-       Nil.
+Program Definition map_nil :=
+  make_rewrite
+    (_ ,, ∙) _
+    (Map · nat_to_tm 0 _ · Nil)
+    Nil.
 
-Definition map_cons
-  := make_rewrite
-       (_ ,, _ ,, _ ,, ∙) _
-       (let f := TmVar Vz in
-        let x := TmVar (Vs Vz) in
-        let xs := TmVar (Vs (Vs Vz)) in
-        Map · f · (Cons · x · xs))
-       (let f := TmVar Vz in
-        let x := TmVar (Vs Vz) in
-        let xs := TmVar (Vs (Vs Vz)) in
-        Cons · (f · x) · (Map · f · xs)).
+Program Definition map_cons :=
+  make_rewrite
+    (_ ,, _ ,, _ ,, ∙) _
+    (Map · nat_to_tm 0 _ · (Cons · nat_to_tm 1 _ · nat_to_tm 2 _))
+    (Cons · (nat_to_tm 0 _ · nat_to_tm 1 _) · (Map · nat_to_tm 0 _ · nat_to_tm 2 _)).
 
 (** The AFS *)
-Definition map_afs
-  := make_afs
-       map_ar
-       (map_nil :: map_cons :: nil).
+Definition map_afs :=
+  make_afs
+    map_ar
+    (map_nil :: map_cons :: nil).
 
 (** The polynomials *)
-Definition map_fun_poly f : poly ∙ (arity map_afs f)
-  := match f with
-     | TNil => P_base (P_const 2)
-     | TCons =>
-       λP let y0 := P_var Vz in
-       λP let y1 := P_var (Vs Vz) in
-       P_base (P_const 3 + y0 + y1)
-     | TMap =>
-       λP let y0 := P_var Vz in
-       λP let G1 := P_var (Vs Vz) in
-       P_base (P_const 3 + P_const 3 * y0 + G1 ·P y0 + P_const 3 * y0 * G1 ·P y0)
-     end.
+Definition map_fun_poly f : poly ∙ (arity map_afs f) :=
+  match f with
+  | TNil => P_base (P_const 2)
+  | TCons =>
+    λP let y0 := P_var Vz in
+    λP let y1 := P_var (Vs Vz) in
+    P_base (P_const 3 + y0 + y1)
+  | TMap =>
+    λP let y0 := P_var Vz in
+    λP let G1 := P_var (Vs Vz) in
+    P_base (P_const 3 + P_const 3 * y0 + G1 ·P y0 + P_const 3 * y0 * G1 ·P y0)
+  end.
 
 (** Strong normalization *)
 Definition map_isSN : isSN map_afs.
